Add hash/hmac to HaclProvider

secure_api/LowCProvider/HaclProvider.ml
@@ -1,8 +1,24 @@
 (* This is a hand-written implementation of HaclProvider.fst. *)
 
-external ocaml_crypto_scalarmult: string -> string -> string -> unit = "ocaml_crypto_scalarmult"
+type hash_alg =
+  | HACL_SHA256
+  | HACL_SHA384
+  | HACL_SHA512
+
+let hash_size = function
+  | HACL_SHA256 -> 32
+  | HACL_SHA384 -> 48
+  | HACL_SHA512 -> 64
+
+external ocaml_crypto_scalarmult: string -> string -> string = "ocaml_crypto_scalarmult"
+external ocaml_crypto_hash: hash_alg -> string -> string = "ocaml_crypto_hash"
+external ocaml_crypto_hmac: hash_alg -> string -> string -> string = "ocaml_crypto_hmac"
 
 let crypto_scalarmult secret point =
-  let out = String.make 32 '\000' in
-  ocaml_crypto_scalarmult out secret point;
-  out
+  ocaml_crypto_scalarmult secret point
+
+let crypto_hash a msg =
+  ocaml_crypto_hash a msg
+
+let crypto_hmac a key msg =
+  ocaml_crypto_hmac a key msg
