secure_api/LowCProvider/lowc_stub.c
@@ -26,6 +26,7 @@
 #include "FStar_UInt128.h"
 #include "Crypto_AEAD_Main_Crypto_Indexing.h"
 #include "Crypto_Symmetric_Bytes.h"
+#include "Crypto_HKDF_Crypto_HMAC.h"
 #include "Curve25519.h"
 #include "FStar.h"
 
@@ -170,11 +171,67 @@ CAMLprim value ocaml_AEAD_decrypt(value state, value iv, value ad,
   CAMLreturn(Val_none);
 }
 
-CAMLprim value ocaml_crypto_scalarmult(value out, value secret, value base) {
-  CAMLparam3(out, secret, base);
+CAMLprim value ocaml_crypto_scalarmult(value secret, value base) {
+  CAMLparam2(secret, base);
+  CAMLlocal1(out);
+  out = caml_alloc_string(32);
   uint8_t *out_p = (uint8_t *) String_val(out);
   uint8_t *secret_p = (uint8_t *) String_val(secret);
   uint8_t *base_p = (uint8_t *) String_val(base);
   Curve25519_crypto_scalarmult(out_p, secret_p, base_p);
-  CAMLreturn(Val_int(0));
+  CAMLreturn(out);
+}
+
+static inline Crypto_HMAC_alg alg_of_int(int i) {
+  switch (i) {
+    case 0:
+      return Crypto_HMAC_SHA256;
+    case 1:
+      return Crypto_HMAC_SHA384;
+    case 2:
+      return Crypto_HMAC_SHA512;
+  }
+  return 0;
+}
+
+static inline size_t hash_size(Crypto_HMAC_alg h) {
+  switch (h) {
+    case Crypto_HMAC_SHA256:
+      return 32;
+    case Crypto_HMAC_SHA384:
+      return 48;
+    case Crypto_HMAC_SHA512:
+      return 64;
+  }
+  return 32;
+}
+
+CAMLprim value ocaml_crypto_hash(value alg, value msg) {
+  CAMLparam2(alg, msg);
+  CAMLlocal1(out);
+
+  Crypto_HMAC_alg h = alg_of_int(Int_val(alg));
+  out = caml_alloc_string(hash_size(h));
+
+  uint8_t *out_p = (uint8_t *) String_val(out);
+  uint8_t *msg_p = (uint8_t *) String_val(msg);
+  Crypto_HMAC_agile_hash(h, out_p, msg_p, caml_string_length(msg));
+  CAMLreturn(out);
+}
+
+CAMLprim value ocaml_crypto_hmac(value alg, value key, value msg) {
+  CAMLparam3(alg, key, msg);
+  CAMLlocal1(out);
+
+  Crypto_HMAC_alg h = alg_of_int(Int_val(alg));
+  out = caml_alloc_string(hash_size(h));
+
+  uint8_t *out_p = (uint8_t *) String_val(out);
+  uint8_t *key_p = (uint8_t *) String_val(key);
+  size_t key_l = caml_string_length(key);
+  uint8_t *msg_p = (uint8_t *) String_val(msg);
+  size_t msg_l = caml_string_length(msg);
+
+  Crypto_HMAC_hmac(h, out_p, key_p, key_l, msg_p, msg_l);
+  CAMLreturn(out);
 }
