secure_api/LowCProvider/fst/HaclProvider.fst
@@ -4,6 +4,27 @@ open FStar.HyperStack.All
 open FStar.Bytes
 
 assume val crypto_scalarmult:
-  secret:lbytes 32 ->
-  point:lbytes 32 ->
+  secret: lbytes 32 ->
+  point: lbytes 32 ->
   EXT (lbytes 32)
+
+type hash_alg =
+  | HACL_SHA256
+  | HACL_SHA384
+  | HACL_SHA512
+
+let hash_size = function
+  | HACL_SHA256 -> 32
+  | HACL_SHA384 -> 48
+  | HACL_SHA512 -> 64
+
+assume val crypto_hash:
+  alg: hash_alg ->
+  msg: bytes ->
+  EXT (lbytes (hash_size alg))
+
+assume val crypto_hmac:
+  alg: hash_alg ->
+  key: bytes ->
+  msg: bytes ->
+  EXT (lbytes (hash_size alg))
